ver2/symbolic_execution_soundness.v
@@ -41,25 +41,268 @@ Import ConcreteInterpreter.
 
 Module SymbolicExecutionSoundness.
 
-Definition eq_con_sym (st: state) (sst: sstate) (ops: stack_op_instr_map) : Prop :=
+
+Lemma eq_execution_states_refl:
+  forall (st: state), eq_execution_states st st.
+Proof.
+  unfold eq_execution_states.
+  intros.
+  rewrite H0. rewrite <- H.
+  rewrite H2. rewrite <- H1.
+  rewrite H4. rewrite <- H3.
+  rewrite H6. rewrite <- H5.
+  intuition. (* this proves the stack and context equivalence *)
+  + unfold eq_memory. intro. reflexivity.
+  + unfold eq_storage. intro. reflexivity.
+Qed.
+
+
+(*
+
+A symbolic state sst is equivalent to a symbolic state st, wrt to an
+initial state init_st, if when instantiating sst using init_st we get
+st' that is equivalent to st. We use eq_execution_states and not '='
+because memory/storage need functional equivalence
+
+*)
+
+Definition st_is_instance_of_sst (init_st st: state) (sst: sstate) (ops: stack_op_instr_map) : Prop :=
   exists (st': state),
-    eval_sstate st sst ops = Some st' /\
+    eval_sstate init_st sst ops = Some st' /\
     eq_execution_states st st'.
   
-  
+(*
+
+A state transformer _tr_ and a symbolic state transformer _str_ are
+equivalent, if when _str_ transforms _sst_ to _sst'_, then for any
+initial state _init_st_ and a state _st_ such that _st_ is an instance
+of _sst_ wrt _init_st_, _tr_ moves from _st_ to _st'_ such that _st'_
+is an instance of _sst'_ wrt _init_st_.
+
+*)
+
 Definition snd_state_transformer ( tr : state -> stack_op_instr_map -> option state ) (symtr : sstate ->  stack_op_instr_map -> option sstate )  : Prop :=
   forall (sst sst': sstate) (ops : stack_op_instr_map),
     symtr sst ops = Some sst' ->
-    forall (st: state),
-      eq_con_sym st sst ops ->
-        exists (st': state), tr st ops = Some st' /\ eq_con_sym st' sst' ops.
+    forall (init_st st: state), st_is_instance_of_sst init_st st sst ops ->
+    exists (st': state), tr st ops = Some st' /\ st_is_instance_of_sst init_st st' sst' ops.
 
 
+(* applying eval_sstack_val on Val w returns Some w *)
+Lemma eval_sstack_val_Val:
+forall (w: EVMWord) (stk: stack) (mem: memory) (strg: storage) (ctx: context)  (bs: sbindings) (ops: stack_op_instr_map),
+    eval_sstack_val (Val w) stk mem strg ctx bs ops = Some w.
+Proof.
+  intros.
+  destruct bs; unfold eval_sstack_val; reflexivity.
+Qed.
+
+(* applying eval_sstack_val on InStackVar i returns (nth_error stk i) *)
+Lemma eval_sstack_val_InStackVar:
+forall (i:nat) (sst: sstate) (stk: stack) (mem: memory) (strg: storage) (ctx: context) (bs: sbindings) (ops: stack_op_instr_map),
+    eval_sstack_val (InStackVar i) stk mem strg ctx bs ops = nth_error stk i.
+Proof.
+  intros.
+  destruct bs; unfold eval_sstack_val; destruct (nth_error stk i); reflexivity; reflexivity.
+Qed.
+
+
+Lemma eval_sstack'_w:
+  forall (w : EVMWord) (sstk: sstack) (stk stk': stack) (mem: memory) (strg: storage) (ctx: context) (sb: sbindings) (ops: stack_op_instr_map),
+    eval_sstack' sstk stk mem strg ctx sb ops = Some stk' ->
+    eval_sstack' ((Val w)::sstk) stk mem strg ctx sb ops = Some (w::stk').
+Proof.
+  intros w sstk stk stk' mem strg ctx sb ops H_eval_sstack'_stk.
+  unfold eval_sstack'.
+  unfold fold_right_option.
+  rewrite eval_sstack_val_Val.
+  unfold eval_sstack' in H_eval_sstack'_stk.
+  unfold fold_right_option in H_eval_sstack'_stk. 
+  rewrite H_eval_sstack'_stk.
+  reflexivity.
+Qed.
+
+
+Lemma eval_sstate_w:
+  forall (w : EVMWord) (sst : sstate) (st st': state) (ops: stack_op_instr_map),
+    eval_sstate st sst ops = Some st' ->
+    eval_sstate st (set_stack_sst sst ((Val w)::(get_stack_sst sst))) ops = Some (set_stack_st st' (w::(get_stack_st st'))).
+Proof.
+  intros.
+  destruct sst eqn:Esst.
+  destruct st eqn:Est.
+  unfold eval_sstate.
+  simpl.
+  unfold eval_sstate in H.
+  simpl in H.
+  unfold eval_sstack in H.
+  simpl in H.
+  destruct (length stk =? instk_height) eqn:El.
+  - destruct sm eqn:Esm.
+    destruct (eval_sstack' sstk stk mem strg ctx map0 ops) eqn:Eevs'.
+    + pose proof (eval_sstack'_w w sstk stk s mem strg ctx map0 ops Eevs').
+      unfold eval_sstack.
+      unfold get_instk_height_sst.
+      rewrite El.
+      unfold get_smap_sst.
+      unfold get_stack_sst.
+      rewrite H0.
+      destruct (eval_smemory stk mem strg ctx (SymExState instk_height sstk smem sstg sctx (SymMap maxid map0)) ops) eqn:Em.
+      ++ destruct (eval_sstorage stk mem strg ctx (SymExState instk_height sstk smem sstg sctx (SymMap maxid map0)) ops) eqn:Es.
+         +++ unfold eval_smemory in Em.
+             unfold get_smap_sst in Em.
+             destruct (fold_right_option
+           (eval_common.EvalCommon.instantiate_memory_update (fun sv : sstack_val => eval_sstack_val sv stk mem strg ctx map0 ops))
+           (get_memory_sst (SymExState instk_height sstk smem sstg sctx (SymMap maxid map0)))) eqn:Efr1.
+             ++++ unfold eval_sstorage in Es.
+                  unfold get_smap_sst in Es.
+                  destruct (fold_right_option
+           (eval_common.EvalCommon.instantiate_storage_update (fun sv : sstack_val => eval_sstack_val sv stk mem strg ctx map0 ops))
+           (get_storage_sst (SymExState instk_height sstk smem sstg sctx (SymMap maxid map0)))) eqn:Efr2.
+                  +++++ unfold eval_smemory.
+                  unfold get_smap_sst.
+                  simpl.
+                  simpl in Efr1.
+                  rewrite Efr1.
+                  unfold eval_sstorage.
+                  unfold get_smap_sst.
+                  simpl.
+                  simpl in Efr2.
+                  rewrite Efr2.
+                  injection H. intros.
+                  rewrite <- H1.
+                  simpl.
+                  injection Es. intros.
+                  injection Em. intros.
+                  rewrite H2.
+                  rewrite H3.
+                  unfold make_st.
+                  reflexivity.
+                  +++++ discriminate.
+             ++++ discriminate.
+         +++ discriminate.
+      ++ discriminate.
+    + discriminate.
+  - discriminate.
+Qed.
+
+Search Nat.eqb.
+Search list.
+
+(*
+Lemma eval_sstack'_len:
+    forall (sstk: sstack) (stk stk': stack) (mem: memory) (strg: storage) (ctx: context) (sb: sbindings) (ops: stack_op_instr_map),
+    eval_sstack' sstk stk mem strg ctx sb ops = Some stk' ->
+    length sstk = length stk'.
+Proof.
+  intros.
+  induction sstk as [|sv sstk' IHsstk'].
+  + simpl in H. injection H. intros. rewrite <- H0. reflexivity.
+  + unfold eval_sstack'  in H.
+ *)
+
+Lemma st_is_instance_of_sst_stk_len:
+  forall (init_st st: state) (sst: sstate) (ops: stack_op_instr_map),
+         st_is_instance_of_sst init_st st sst ops ->
+         length (get_stack_sst sst) = length (get_stack_st st) /\
+         length (get_stack_st init_st) = get_instk_height_sst sst.
+Proof.
+  intros.
+  unfold st_is_instance_of_sst in H.
+  destruct H as [st'].
+  destruct H.
+  unfold eval_sstate in H. unfold eval_sstack in H.
+  destruct (length (get_stack_st init_st) =? get_instk_height_sst sst) eqn:E0.
+  + apply beq_nat_true in E0.
+    split.
+    ++ destruct (get_smap_sst sst).
+       destruct (eval_sstack' (get_stack_sst sst) (get_stack_st init_st) (get_memory_st init_st) (get_storage_st init_st) 
+                   (get_context_st init_st) map0 ops) eqn:Levs'.
+       +++ destruct (eval_smemory (get_stack_st init_st) (get_memory_st init_st) (get_storage_st init_st) (get_context_st init_st) sst ops) eqn:E1.
+           ++++ destruct (eval_sstorage (get_stack_st init_st) (get_memory_st init_st) (get_storage_st init_st) (get_context_st init_st) sst ops) eqn:E2.
+                +++++ injection H.
+                intros.
+                unfold eval_sstack' in Levs'.
+                apply fold_right_option_len in Levs'.
+                destruct st eqn:Est.
+                destruct init_st eqn:Eist.
+                unfold eq_execution_states in H0.
+                simpl.
+                rewrite <- H1 in H0.
+                simpl in H0. 
+                destruct H0 with (stk1:=stk)(stk2:=s)(mem1:=mem)(mem2:=m)(strg1:=strg)(strg2:=s0)(ctx1:=ctx)(ctx2:=ctx0).
+                reflexivity. reflexivity. reflexivity. reflexivity. reflexivity.
+                reflexivity. reflexivity. reflexivity.
+                unfold eq_stack in H2. rewrite H2. apply Levs'.
+                +++++ discriminate.
+           ++++ discriminate.
+       +++ discriminate.
+    ++ apply E0.
+  + discriminate.
+Qed.
 
 Lemma push_snd:
-  forall w, snd_state_transformer (push_c w) (push_s w).       
+  forall w, snd_state_transformer (push_c w) (push_s w).
 Proof.
-Admitted.
+intro w.
+  unfold snd_state_transformer.
+  intros.
+  pose proof (st_is_instance_of_sst_stk_len init_st st sst ops H0) as H1.
+  destruct H1.
+  unfold push_s in H.
+  unfold push in H.
+  destruct (length (get_stack_sst sst) <? StackSize) eqn:E0.
+  -  exists (set_stack_st st (w::(get_stack_st st))).
+     unfold push_c.
+     unfold push.
+     rewrite <- H1.
+     rewrite E0.
+     split.
+     + reflexivity.
+     + unfold st_is_instance_of_sst in H0.
+       destruct H0 as [st'].
+       destruct H0.
+       injection H. intros.
+       unfold st_is_instance_of_sst.
+       exists (set_stack_st st' (w::(get_stack_st st'))).
+       split.
+       ++ pose proof (eval_sstate_w w sst init_st st' ops H0).
+          rewrite H4 in H5. rewrite H5.
+          reflexivity.
+       ++ destruct st eqn:Est.
+          destruct st' eqn:Est'.
+          simpl.
+          unfold eq_execution_states in H3.
+          simpl in H3.
+          pose proof (H3 stk stk0 mem mem0 strg strg0 ctx ctx0).
+          destruct H5.
+          reflexivity.
+          reflexivity.
+          reflexivity.
+          reflexivity.
+          reflexivity.
+          reflexivity.
+          reflexivity.
+          reflexivity.
+          destruct H6.
+          destruct H7.
+          unfold eq_execution_states. simpl. intros.
+          rewrite H9.
+          rewrite H10.
+          rewrite H11.
+          rewrite H12.
+          rewrite H13.
+          rewrite H14.
+          rewrite H15.
+          rewrite H16.
+          split.
+          +++ unfold eq_stack.
+              unfold eq_stack in H5.
+              rewrite H5.
+              reflexivity.
+          +++ split. apply H6. split. apply H7. apply H8.
+  - discriminate.
+Qed.  
 
 Lemma pop_snd:
   snd_state_transformer pop_c pop_s.       
@@ -131,35 +374,281 @@ Proof.
   - unfold evm_exec_instr_c. unfold evm_exec_instr_s. apply exec_stack_op_intsr_snd.
 Qed.
 
-  
+
+(* evm_exec_block_s and evm_exec_block_c are sound transformers -- when applied to p *)
 Lemma evm_exec_block_snd:
   forall (p : block),
     snd_state_transformer (evm_exec_block_c p) (evm_exec_block_s p).
 Proof.
   unfold snd_state_transformer.
-  induction p as [| i p' IHp'].
-  - intros. simpl. exists st. split.
+  induction p as [| i p' IHp']. (* induction of the length of the block p *)
+
+  - simpl. (* execute the empty block -- in several places *)
+    intros sst sst' ops H_sexec_nil.
+    intros init_st st H_st_inst_sst.
+    exists st. (* we use st since p=[], i.e., we don't execute anything *)
+    split. (* split the conjuction into two goals *)
     + reflexivity.
-    + injection H as H1. rewrite <- H1. apply H0.
-  - intros. unfold evm_exec_block_s in H. fold evm_exec_block_s in H.
-    destruct (evm_exec_instr_s i sst ops) eqn:E.
-    + apply evm_exec_instr_snd in E as E0. destruct E0 with (st:=st). apply H0.
-      apply IHp' with (st:=x) in H.
-      * destruct H. exists x0. split.
-        ** unfold evm_exec_block_c. destruct H1. rewrite H1. fold evm_exec_block_c. destruct H. apply H.
-        ** destruct H. apply H2.
-      * destruct H1. apply H2.
-    + discriminate H.
+    + injection H_sexec_nil as H_sst_eq_sst' (* infer that sst and sst' are equal *).
+      rewrite <- H_sst_eq_sst'. (* replace sst' by sst in the goal *)
+      apply H_st_inst_sst. (* the goal is the assumption H_st_inst_sst *)
+
+  - intros sst sst' ops H_sexec_ip' init_st st H_st_inst_sst.
+
+    (* unfold the symbolic execution of i::p' and fold the recursive call *)
+    unfold evm_exec_block_s in H_sexec_ip'. 
+    fold evm_exec_block_s in H_sexec_ip'.
+
+    (* we split on the result of symbolically executiing i: Some sst'' or None *)
+    destruct (evm_exec_instr_s i sst ops) as [sst''|] eqn:E_evm_exec_instr_s.
+
+    (* the case of Some sst'' *)
+    +
+      (* derive relation between execution and symbolic execution of i *)
+      apply evm_exec_instr_snd with (i:=i) in E_evm_exec_instr_s as E_evm_exec_instr_s_0.
+      pose proof (E_evm_exec_instr_s_0 init_st st H_st_inst_sst) as E_evm_exec_instr_c.
+
+      (* choose a value for exists st' and split the resulting conjunction *)
+      destruct E_evm_exec_instr_c as [st' E_evm_exec_instr_c_st']. 
+      destruct E_evm_exec_instr_c_st' as [E_evm_exec_instr_c_st'_left E_evm_exec_instr_c_st'_right].
+      
+      (* apply the induction hypothesis for symbolically exexuting p'
+      from sst'' (the result of executing i) to st'. Use H_sexec_ip'
+      for the premise that symbolic execution of p' succeeds *)
+      pose proof (IHp' sst'' sst' ops H_sexec_ip') as IHp'_sst''_sst'.
+
+      (* Now we derive the concrete execution of p' and solut the resulting conjunction *)
+      pose proof (IHp'_sst''_sst' init_st st' E_evm_exec_instr_c_st'_right) as H_evm_exec_block_c_p'.
+      destruct H_evm_exec_block_c_p' as [st'' H_evm_exec_block_c_p'_st''].
+      destruct H_evm_exec_block_c_p'_st'' as [H_evm_exec_block_c_p'_st''_left H_evm_exec_block_c_p'_st''_right].
+
+      (* choose a value for the existential variable in the goal and
+      split the conjunction into two goals*)
+      exists st''.
+      split.
+      
+      * unfold evm_exec_block_c. (* unfold execution of i::p' *)
+        rewrite E_evm_exec_instr_c_st'_left. (* use the assumption on the result of executing i *)
+        fold evm_exec_block_c. (* fold the recursive call *)
+        apply H_evm_exec_block_c_p'_st''_left. (* the goal is an assumption *)
+        
+      * apply H_evm_exec_block_c_p'_st''_right. (* the goal is an assumption *)
+
+    (* The case of None *)
+    + discriminate H_sexec_ip'.
 Qed.
 
 
-Theorem gen_empty_sstate_snd:
+
+(* The instk_height of the symbolic state (gen_empty_sstate instk_height) is instk_height *)
+Lemma instkh_gen_empty_instkh:
+  forall instk_height,
+    get_instk_height_sst (gen_empty_sstate instk_height) = instk_height.
+Proof.
+  intros. reflexivity.
+Qed.
+
+Search sub.
+
+(* when i < length l, the access (nth_error l i) suceeds *)
+Lemma nth_error_ok' :
+  forall (T: Type) (l : list T) (i : nat),
+    i < length l -> 
+    exists (v: T), nth_error l i = Some v.
+Proof.
+  intros T l i. revert T l.
+  induction i as [| i' IH].
+  - intros T l Hlen.
+    destruct l as [| h t] eqn: eq_l.
+    + simpl in Hlen. 
+      pose proof (Nat.nlt_0_r 0). contradiction.
+    + simpl. exists h. reflexivity.
+  - intros T l Hlen.
+    destruct l as [| h t] eqn: eq_l.
+    + simpl in Hlen. pose proof (Nat.nlt_0_r (S i')). contradiction.
+    + simpl in Hlen. rewrite <- Nat.succ_lt_mono in Hlen.
+      simpl.
+      pose proof (IH T t Hlen). assumption.
+Qed.
+
+(* if m<n then 0<n-m *)
+Lemma lt_minus_lt_0: forall (n m: nat),
+m < n -> 0 < (n - m).
+Proof.
+  intuition.
+(*
+intros n.
+induction n as [| n' IH].
+- intros m Hm_lt_0. 
+  pose proof (Nat.nlt_0_r m).
+  contradiction.
+- intros m Hm_lt_sn.
+  destruct m as [|m'] eqn: eq_m.
+  + rewrite -> Nat.sub_0_r. assumption.
+  + pose proof (lt_S_n m' n' Hm_lt_sn) as eq_m'_lt_n'.
+    pose proof (IH m' eq_m'_lt_n') as IHc.
+    rewrite -> Nat.sub_succ.
+    assumption.
+*)
+Qed.
+
+(* when i<n, (n-(i+1))+1=n-i *)
+Lemma succ_minus_succ: forall (n i: nat),
+i < n -> S (n - S i) = n - i.
+Proof.
+  intuition.
+(*
+intros n i H_i_lt_n.
+rewrite -> Nat.sub_succ_r.
+pose proof (lt_minus_lt_0 n i H_i_lt_n) as Hni_gt_0.
+pose proof (Nat.succ_pred_pos (n - i) Hni_gt_0) as Hs_pred_n_i.
+assumption.
+*)
+Qed.
+
+(* if the i-th element is v, skipping i element we get v::(skipping i+1 elements) *)
+Lemma skipn_nth:
+  forall (T: Type) (i: nat) (l: list T) (v: T),
+    nth_error l i = Some v -> 
+    skipn i l = v :: (skipn (S i) l).
+Proof.
+  intros T i. induction i as [| i' IH].
+  - intros l v Hnth_error.
+    destruct l as [|h t] eqn: eq_l.
+    + simpl in Hnth_error. discriminate.
+    + simpl in Hnth_error. simpl.
+      injection Hnth_error. intros eq_h_v. rewrite -> eq_h_v.
+      reflexivity.
+  - intros l v Hnth_error.
+    destruct l as [|h t] eqn: eq_l.
+    + simpl in Hnth_error. discriminate.
+    + simpl in Hnth_error.
+      rewrite -> skipn_cons.
+      rewrite -> skipn_cons.
+      pose proof (IH t v Hnth_error).
+      assumption.
+Qed.
+
+Lemma gen_empty_sstate_eval_sstack'_snd:
+  forall (i n : nat) (stk: stack) (mem: memory) (strg: storage) (ctx: context)  (bs: sbindings) (ops : stack_op_instr_map),
+    length stk = n ->
+    i <= n ->
+    n >= 0 ->
+    eval_sstack' (List.map InStackVar (seq (n-i) i)) stk mem strg ctx bs ops = Some (skipn (n-i) stk).
+Proof.
+  intros.
+  induction i as [|i' IHi'].
+  - simpl. rewrite -> Nat.sub_0_r. rewrite <- H. rewrite -> skipn_all. reflexivity.
+  - destruct bs.
+    simpl.
+    pose proof (gt_Sn_O i') as eq_Si_gt_0.
+    pose proof (Nat.sub_lt n (S i') H0 eq_Si_gt_0) as eq_si_n.
+    rewrite <- H in eq_si_n at 2.
+    pose proof (@nth_error_ok' EVMWord stk (n - S i') eq_si_n) as
+      eq_nth_error_value_ex.
+    destruct eq_nth_error_value_ex. rewrite H2.
+  pose proof (succ_minus_succ n i' H0) as eq_n_i_succ.
+  rewrite eq_n_i_succ.
+  pose proof (le_Sn_le i' n H0) as eq_i'_leq_n.
+  apply IHi' in eq_i'_leq_n.
+  rewrite eq_i'_leq_n.
+  pose proof (skipn_nth EVMWord (n - (S i')) stk x H2) as eq_skipn_x.
+  rewrite eq_skipn_x.
+  rewrite eq_n_i_succ. reflexivity.
+  (* this is repetition of the above, should be rewritten using ; *)
+    simpl.
+    pose proof (gt_Sn_O i') as eq_Si_gt_0.
+    pose proof (Nat.sub_lt n (S i') H0 eq_Si_gt_0) as eq_si_n.
+    rewrite <- H in eq_si_n at 2.
+    pose proof (@nth_error_ok' EVMWord stk (n - S i') eq_si_n) as
+      eq_nth_error_value_ex.
+    destruct eq_nth_error_value_ex. rewrite H2.
+  pose proof (succ_minus_succ n i' H0) as eq_n_i_succ.
+  rewrite eq_n_i_succ.
+  pose proof (le_Sn_le i' n H0) as eq_i'_leq_n.
+  apply IHi' in eq_i'_leq_n.
+  rewrite eq_i'_leq_n.
+  pose proof (skipn_nth EVMWord (n - (S i')) stk x H2) as eq_skipn_x.
+  rewrite eq_skipn_x.
+  rewrite eq_n_i_succ. reflexivity.  
+Qed.
+
+
+Lemma gen_empty_sstate_eval_sstack_snd:
+  forall (n : nat) (stk: stack) (mem: memory) (strg: storage) (ctx: context) (sst: sstate) (sstk: sstack) (ops : stack_op_instr_map),
+    length stk = n ->
+    sst = (gen_empty_sstate n) ->
+    sstk = (get_stack_sst sst) -> 
+    eval_sstack stk mem strg ctx sst ops = Some stk.
+Proof.
+  intros.
+  unfold eval_sstack.
+  rewrite H0.
+  rewrite instkh_gen_empty_instkh. rewrite H. rewrite Nat.eqb_refl.
+  destruct (get_smap_sst (gen_empty_sstate n)).
+  rewrite <- H0.
+  rewrite <- H1.
+  pose proof (gen_empty_sstate_eval_sstack'_snd n n stk mem strg ctx map0 ops).
+  apply H2 in H.
+  unfold gen_empty_sstate in H0. unfold make_sst in H0. rewrite H0 in H1. simpl in H1. rewrite H1.
+  rewrite Nat.sub_diag in H. unfold skipn in H. apply H. apply le_n.
+  destruct n.
+  + apply le_n.
+  + apply le_0_n.
+Qed.
+
+Lemma gen_empty_sstate_eval_smemory_snd:
+  forall (stk: stack) (mem: memory) (strg: storage) (ctx: context) (instk_height: nat) (sst: sstate) (ops : stack_op_instr_map),
+    sst = gen_empty_sstate instk_height ->
+    eval_smemory stk mem strg ctx sst ops = Some mem.
+Proof.
+  intros.
+  
+  unfold gen_empty_sstate in H. unfold make_sst in H. unfold eval_smemory.
+  unfold get_smap_sst. rewrite H. unfold empty_smap.
+  unfold get_memory_sst. unfold empty_smemory.
+  unfold fold_right_option.
+  unfold eval_common.EvalCommon.update_memory. reflexivity.
+Qed.
+
+Lemma gen_empty_sstate_eval_sstorage_snd:
+  forall (stk: stack) (mem: memory) (strg: storage) (ctx: context) (instk_height: nat) (sst: sstate) (ops : stack_op_instr_map),
+    sst = gen_empty_sstate instk_height ->
+    eval_sstorage stk mem strg ctx sst ops = Some strg.
+Proof.
+  intros.
+  unfold gen_empty_sstate in H. unfold make_sst in H. unfold eval_sstorage.
+  unfold get_smap_sst. rewrite H. unfold empty_smap.
+  unfold get_storage_sst. unfold empty_sstorage.
+  unfold fold_right_option.
+  unfold eval_common.EvalCommon.update_storage. reflexivity.
+Qed.
+
+(* An initial symbolic state is equivalent to any state, as long as
+they refer to a stack with the same size *)
+Lemma gen_empty_sstate_snd:
   forall (st: state) (instk_height: nat) (sst: sstate) (ops : stack_op_instr_map),
     length (get_stack_st st) = instk_height ->
     sst = gen_empty_sstate instk_height ->
-    eq_con_sym st sst ops.
+    st_is_instance_of_sst st st sst ops.
 Proof.
-Admitted.
+  intros.
+  unfold st_is_instance_of_sst.
+  exists st.
+  split.
+  + unfold eval_sstate.
+    assert(H1:=H0).
+    assert(H2:=H0).
+    pose proof (gen_empty_sstate_eval_sstack_snd instk_height (get_stack_st st) (get_memory_st st) (get_storage_st st) (get_context_st st) sst (get_stack_sst sst)) ops as E.
+    apply E in H0.
+    apply E in H. rewrite H.
+    apply gen_empty_sstate_eval_smemory_snd with (stk:=(get_stack_st st))(mem:=(get_memory_st st))(strg:=(get_storage_st st))(ctx:=(get_context_st st))(ops:=ops) in H1. rewrite H1.
+    apply gen_empty_sstate_eval_sstorage_snd with (stk:=(get_stack_st st))(mem:=(get_memory_st st))(strg:=(get_storage_st st))(ctx:=(get_context_st st))(ops:=ops) in H2. rewrite H2.
+    destruct st. reflexivity.
+    apply H1.
+    reflexivity. apply H. reflexivity.
+   + apply eq_execution_states_refl.
+Qed.
 
 Theorem symbolic_exec_snd:
   forall (p : block) (instk_height : nat) (sst : sstate) (ops : stack_op_instr_map),
@@ -168,7 +657,7 @@ Theorem symbolic_exec_snd:
       length (get_stack_st st) = instk_height -> 
       exists (st': state),
         evm_exec_block_c p st ops = Some st' /\
-          eq_con_sym st' sst ops. 
+          st_is_instance_of_sst st st' sst ops. 
 Proof.
   intros.
   unfold evm_sym_exec in H.
