ver2/symbolic_state_eval.v
@@ -34,14 +34,13 @@ Module SymbolicStateEval.
 
 
 
-Fixpoint eval_sstack_val (sv : sstack_val) (st: state) (sb: sbindings) (ops: stack_op_instr_map) : option EVMWord :=  
+Fixpoint eval_sstack_val (sv : sstack_val) (stk : stack) (mem: memory) (strg: storage) (ctx: context) (sb: sbindings) (ops: stack_op_instr_map) : option EVMWord :=  
   match sv with
   (* Concrere values are retuned *)
   | Val v => Some v
 
   (* A stack element 'InStackVar n' takes its value from the n-th element of the concrete stack *)                  
   | InStackVar n =>
-      let stk := get_stack_st st in
       match nth_error stk n with
       | Some v => Some v
       | None => None
@@ -59,7 +58,7 @@ Fixpoint eval_sstack_val (sv : sstack_val) (st: state) (sb: sbindings) (ops: sta
             match smv with
 
             (* basic value: we just evaluate 'v' recursively, it is a stack element *)
-            | SymBasicVal v => eval_sstack_val v st sb' ops
+            | SymBasicVal v => eval_sstack_val v stk mem strg ctx sb' ops
 
             (* stack operation instruction: we evaluate the argument
             recursively and then evaluate the corresponding operation *)
@@ -68,10 +67,10 @@ Fixpoint eval_sstack_val (sv : sstack_val) (st: state) (sb: sbindings) (ops: sta
                 | OpImp nargs f _ =>
                      (* first check that the number of argumets agree with what is declared in the map *)
                     if (List.length args =? nargs) then
-                      let f_eval_list := fun (sv': sstack_val) => eval_sstack_val sv' st sb' ops in
+                      let f_eval_list := fun (sv': sstack_val) => eval_sstack_val sv' stk mem strg ctx sb' ops in
                       match fold_right_option f_eval_list args with
                       | None => None
-                      | Some vargs => Some (f (get_context_st st) vargs)
+                      | Some vargs => Some (f ctx vargs)
                       end
                     else None
                 end
@@ -83,14 +82,14 @@ Fixpoint eval_sstack_val (sv : sstack_val) (st: state) (sb: sbindings) (ops: sta
                 4. look for the desired value in the memory 
              *)
             | SymMLOAD soffset smem =>
-                let f_eval_mem_update := instantiate_memory_update (fun sv => eval_sstack_val sv st sb' ops) in
+                let f_eval_mem_update := instantiate_memory_update (fun sv => eval_sstack_val sv stk mem strg ctx sb' ops) in
                 match fold_right_option f_eval_mem_update smem with (* Evaluate the arguments of the updates *)
                 | None => None
                 | Some mem_updates =>
-                    match eval_sstack_val soffset st sb' ops with (* Evaluate the offset *)
+                    match eval_sstack_val soffset stk mem strg ctx sb' ops with (* Evaluate the offset *)
                     | None => None
                     | Some offset =>
-                        let mem := update_memory (get_memory_st st) mem_updates in (* apply updates to the memory *)
+                        let mem := update_memory mem mem_updates in (* apply updates to the memory *)
                         Some (mload mem offset) (* lookup for the desired value in the memory *)
                     end
                 end
@@ -102,14 +101,14 @@ Fixpoint eval_sstack_val (sv : sstack_val) (st: state) (sb: sbindings) (ops: sta
                 4. look for the desired value in the stroarge 
              *)
             | SymSLOAD skey sstrg =>
-                let f_eval_strg_update := instantiate_storage_update (fun sv => eval_sstack_val sv st sb' ops) in
+                let f_eval_strg_update := instantiate_storage_update (fun sv => eval_sstack_val sv stk mem strg ctx sb' ops) in
                 match fold_right_option f_eval_strg_update sstrg with (* Evaluate the arguments of the updates *)
                 | None => None
                 | Some strg_updates =>
-                    match eval_sstack_val skey st sb' ops with (* Evaluate the key *)
+                    match eval_sstack_val skey stk mem strg ctx sb' ops with (* Evaluate the key *)
                     | None => None
                     | Some key =>
-                        let strg := update_storage (get_storage_st st) strg_updates in (* apply updates to the storage *)
+                        let strg := update_storage strg strg_updates in (* apply updates to the storage *)
                         Some (sload strg key) (* lookup for the desired value in the storage *)
                     end
                 end
@@ -121,65 +120,65 @@ Fixpoint eval_sstack_val (sv : sstack_val) (st: state) (sb: sbindings) (ops: sta
                 4. apply the SHA3 function that is given in the context 
              *)
             | SymSHA3 soffset ssize smem =>
-                let f_eval_mem_update := instantiate_memory_update (fun sv => eval_sstack_val sv st sb' ops) in
+                let f_eval_mem_update := instantiate_memory_update (fun sv => eval_sstack_val sv stk mem strg ctx sb' ops) in
                 match fold_right_option f_eval_mem_update smem with (* Evaluate the arguments of the updates *)
                 | None => None
                 | Some mem_updates =>
-                    match eval_sstack_val soffset st sb' ops with (* Evaluate the offset *)
+                    match eval_sstack_val soffset stk mem strg ctx sb' ops with (* Evaluate the offset *)
                     | None => None
                     | Some offset =>
-                        match eval_sstack_val ssize st sb' ops with (* Evaluate the size *)
+                        match eval_sstack_val ssize stk mem strg ctx sb' ops with (* Evaluate the size *)
                         | None => None
                         | Some size =>
-                            let mem := update_memory (get_memory_st st) mem_updates in (* apply updates to the memory *)
-                            let f_sha3 := (get_keccak256_ctx (get_context_st st)) in (* get the sha3 function from the context and ... *)
+                            let mem := update_memory mem mem_updates in (* apply updates to the memory *)
+                            let f_sha3 := (get_keccak256_ctx ctx) in (* get the sha3 function from the context and ... *)
                             Some (f_sha3 mem offset size) (* ... apply it to the corresponding data *)
                         end
                     end
                 end
             end
-          else eval_sstack_val sv st sb' ops   (* The fresh variable is not the first in the binding so we continue recursively with the rest of bindings *)
+          else eval_sstack_val sv stk mem strg ctx sb' ops   (* The fresh variable is not the first in the binding so we continue recursively with the rest of bindings *)
       end
   end.
 
 
 
-Definition eval_sstack (st: state) (sst: sstate) (ops: stack_op_instr_map) : option stack :=
-  let stk := get_stack_st st in
+Definition eval_sstack' (sstk: sstack) (stk: stack) (mem: memory) (strg: storage) (ctx: context) (sb: sbindings) (ops: stack_op_instr_map) : option stack :=
+  fold_right_option (fun sv => eval_sstack_val sv stk mem strg ctx sb ops) sstk.
+
+Definition eval_sstack (stk: stack) (mem: memory) (strg: storage) (ctx: context) (sst: sstate) (ops: stack_op_instr_map) : option stack :=
   let instk_height := (get_instk_height_sst sst) in
   if (length stk) =? instk_height then
     let sstk := get_stack_sst sst in
     match (get_smap_sst sst) with
-    | SymMap _ sb => fold_right_option (fun sv => eval_sstack_val sv st sb ops) sstk 
+    | SymMap _ sb => eval_sstack' sstk stk mem strg ctx sb ops 
     end
   else
     None.
 
 
 
-Definition eval_smemory (st: state) (sst: sstate) (ops: stack_op_instr_map) : option memory :=
+Definition eval_smemory (stk: stack) (mem: memory) (strg: storage) (ctx: context) (sst: sstate) (ops: stack_op_instr_map) : option memory :=
   match get_smap_sst sst with
   | SymMap _ sb =>
-      let f_eval_mem_update := instantiate_memory_update (fun sv => eval_sstack_val sv st sb ops) in
+      let f_eval_mem_update := instantiate_memory_update (fun sv => eval_sstack_val sv stk mem strg ctx sb ops) in
       let smem := get_memory_sst sst in
       match fold_right_option f_eval_mem_update smem with
       | None => None
       | Some updates =>
-          let mem := (get_memory_st st) in
           let mem' := update_memory mem updates in
           Some mem'
       end
   end.
 
-Definition eval_sstorage (st: state) (sst: sstate) (ops: stack_op_instr_map) : option storage :=
+Definition eval_sstorage (stk: stack) (mem: memory) (strg: storage) (ctx: context) (sst: sstate) (ops: stack_op_instr_map) : option storage :=
   match get_smap_sst sst with
   | SymMap _ sb =>
-      let f_eval_strg_update := instantiate_storage_update (fun sv => eval_sstack_val sv st sb ops) in
+      let f_eval_strg_update := instantiate_storage_update (fun sv => eval_sstack_val sv stk mem strg ctx sb ops) in
       let sstrg := get_storage_sst sst in
       match fold_right_option f_eval_strg_update sstrg with
       | None => None
       | Some updates =>
-          let strg := (get_storage_st st) in
           let strg' := update_storage strg updates in
           Some strg'
       end
@@ -187,17 +186,20 @@ Definition eval_sstorage (st: state) (sst: sstate) (ops: stack_op_instr_map) : o
 
 
 Definition eval_sstate (st: state) (sst: sstate) (ops: stack_op_instr_map) : option state :=
-  match eval_sstack st sst ops with
+  let stk := get_stack_st st in
+  let mem := get_memory_st st in
+  let strg := get_storage_st st in
+  let ctx := get_context_st st in
+  match eval_sstack stk mem strg ctx sst ops with
   | None => None
-  | Some stk =>
-      match eval_smemory st sst ops with
+  | Some stk' =>
+      match eval_smemory stk mem strg ctx sst ops with
       | None => None
-      | Some mem =>
-          match eval_sstorage st sst ops with
+      | Some mem' =>
+          match eval_sstorage stk mem strg ctx sst ops with
           | None => None
-          | Some strg =>
-              let ctx := get_context_st st in
-              let sst' := make_st stk mem strg ctx in
+          | Some strg' =>
+              let sst' := make_st stk' mem' strg' ctx in
               Some sst'
           end
       end
